<?xml version="1.0"?>
<rdf:RDF xmlns="http://www.semanticweb.org/paulagranadosgarcia/CuCoO_revised#"
     xml:base="http://www.semanticweb.org/paulagranadosgarcia/CuCoO_revised"
     xmlns:rdf="http://www.w3.org/1999/02/22-rdf-syntax-ns#"
     xmlns:owl="http://www.w3.org/2002/07/owl#"
     xmlns:xml="http://www.w3.org/XML/1998/namespace"
     xmlns:xsd="http://www.w3.org/2001/XMLSchema#"
     xmlns:rdfs="http://www.w3.org/2000/01/rdf-schema#">
    <owl:Ontology rdf:about="http://www.semanticweb.org/paulagranadosgarcia/CuCoO">
        <rdfs:comment>This ontology defines main concepts related to cross-culutral contact in antiquity. This ontology is distributed under a Creative Commons Attribution License - https://creativecommons.org/licenses/by-sa/2.0/uk/deed.en_GB.</rdfs:comment>
    </owl:Ontology>
    


    <!-- 
    ///////////////////////////////////////////////////////////////////////////////////////
    //
    // Object Properties
    //
    ///////////////////////////////////////////////////////////////////////////////////////
     -->

    


    <!-- http://www.semanticweb.org/paulagranadosgarcia/CuCoO/ShowsAccesories -->

    <owl:ObjectProperty rdf:about="http://www.semanticweb.org/paulagranadosgarcia/CuCoO/ShowsAccesories">
        <rdfs:subPropertyOf rdf:resource="http://www.semanticweb.org/paulagranadosgarcia/CuCoO/ShowsPhysicalAppearance"/>
    </owl:ObjectProperty>
    


    <!-- http://www.semanticweb.org/paulagranadosgarcia/CuCoO/ShowsHairstyle -->

    <owl:ObjectProperty rdf:about="http://www.semanticweb.org/paulagranadosgarcia/CuCoO/ShowsHairstyle">
        <rdfs:subPropertyOf rdf:resource="http://www.semanticweb.org/paulagranadosgarcia/CuCoO/ShowsPhysicalAppearance"/>
        <rdfs:comment>Relates a person with the hair style they display</rdfs:comment>
    </owl:ObjectProperty>
    


    <!-- http://www.semanticweb.org/paulagranadosgarcia/CuCoO/ShowsPhysicalAppearance -->

    <owl:ObjectProperty rdf:about="http://www.semanticweb.org/paulagranadosgarcia/CuCoO/ShowsPhysicalAppearance">
        <rdfs:subPropertyOf rdf:resource="http://www.semanticweb.org/paulagranadosgarcia/CuCoO/hasTrait"/>
        <rdfs:domain rdf:resource="http://www.semanticweb.org/paulagranadosgarcia/CuCoO/Person"/>
        <rdfs:range rdf:resource="http://www.semanticweb.org/paulagranadosgarcia/CuCoO/PhysicalAppearance"/>
        <rdfs:comment>Relates a person with the physical appearance it displays.</rdfs:comment>
    </owl:ObjectProperty>
    


    <!-- http://www.semanticweb.org/paulagranadosgarcia/CuCoO/ShowsPosture -->

    <owl:ObjectProperty rdf:about="http://www.semanticweb.org/paulagranadosgarcia/CuCoO/ShowsPosture">
        <rdfs:subPropertyOf rdf:resource="http://www.semanticweb.org/paulagranadosgarcia/CuCoO/ShowsPhysicalAppearance"/>
        <rdfs:comment>Relates a person with the posture they display.</rdfs:comment>
    </owl:ObjectProperty>
    


    <!-- http://www.semanticweb.org/paulagranadosgarcia/CuCoO/Wears -->

    <owl:ObjectProperty rdf:about="http://www.semanticweb.org/paulagranadosgarcia/CuCoO/Wears">
        <rdfs:subPropertyOf rdf:resource="http://www.semanticweb.org/paulagranadosgarcia/CuCoO/ShowsPhysicalAppearance"/>
        <rdfs:domain rdf:resource="http://www.semanticweb.org/paulagranadosgarcia/CuCoO/Person"/>
        <rdfs:range rdf:resource="http://www.semanticweb.org/paulagranadosgarcia/CuCoO/Clothes"/>
        <rdfs:comment>Relates a person with the clothes they wear.</rdfs:comment>
    </owl:ObjectProperty>
    


    <!-- http://www.semanticweb.org/paulagranadosgarcia/CuCoO/hasAdministrativeOrganisation -->

    <owl:ObjectProperty rdf:about="http://www.semanticweb.org/paulagranadosgarcia/CuCoO/hasAdministrativeOrganisation">
        <rdfs:domain rdf:resource="http://www.semanticweb.org/paulagranadosgarcia/CuCoO/Settlement"/>
        <rdfs:range rdf:resource="http://www.semanticweb.org/paulagranadosgarcia/CuCoO/SettlementAdministrativeOrganisation"/>
        <rdfs:comment>Relates a settlement with its Administrative Organisation.</rdfs:comment>
    </owl:ObjectProperty>
    


    <!-- http://www.semanticweb.org/paulagranadosgarcia/CuCoO/hasAspect -->

    <owl:ObjectProperty rdf:about="http://www.semanticweb.org/paulagranadosgarcia/CuCoO/hasAspect">
        <rdfs:domain rdf:resource="http://www.semanticweb.org/paulagranadosgarcia/CuCoO/CulturalContactAgent"/>
        <rdfs:range rdf:resource="http://www.semanticweb.org/paulagranadosgarcia/CuCoO/CulturalContactAspects"/>
        <rdfs:comment>Relates a CulutralContactAgent (e.g. coin) with the CulutralContactAspect featured (e.g. Linguistic).</rdfs:comment>
    </owl:ObjectProperty>
    


    <!-- http://www.semanticweb.org/paulagranadosgarcia/CuCoO/hasCarving -->

    <owl:ObjectProperty rdf:about="http://www.semanticweb.org/paulagranadosgarcia/CuCoO/hasCarving">
        <rdfs:subPropertyOf rdf:resource="http://www.semanticweb.org/paulagranadosgarcia/CuCoO/hasTrait"/>
        <rdfs:domain rdf:resource="http://www.semanticweb.org/paulagranadosgarcia/CuCoO/Thing"/>
        <rdfs:range rdf:resource="http://www.semanticweb.org/paulagranadosgarcia/CuCoO/Carving"/>
        <rdfs:comment>Relates an object with the type of carving that it displays (e.g. low relief).</rdfs:comment>
    </owl:ObjectProperty>
    


    <!-- http://www.semanticweb.org/paulagranadosgarcia/CuCoO/hasContent -->

    <owl:ObjectProperty rdf:about="http://www.semanticweb.org/paulagranadosgarcia/CuCoO/hasContent">
        <rdfs:subPropertyOf rdf:resource="http://www.semanticweb.org/paulagranadosgarcia/CuCoO/hasTrait"/>
        <rdfs:domain rdf:resource="http://www.semanticweb.org/paulagranadosgarcia/CuCoO/Text"/>
        <rdfs:comment>Relates any type of text with its content.</rdfs:comment>
    </owl:ObjectProperty>
    


    <!-- http://www.semanticweb.org/paulagranadosgarcia/CuCoO/hasContext -->

    <owl:ObjectProperty rdf:about="http://www.semanticweb.org/paulagranadosgarcia/CuCoO/hasContext">
        <rdfs:domain rdf:resource="http://www.semanticweb.org/paulagranadosgarcia/CuCoO/CulturalContactAgent"/>
        <rdfs:range rdf:resource="http://www.semanticweb.org/paulagranadosgarcia/CuCoO/CulturalContactContext"/>
        <rdfs:comment>Relates a CulturalConceptAgent (e.g. sculpture) with the CulturalContact Context whose finding is related to (e.g. war).</rdfs:comment>
    </owl:ObjectProperty>
    


    <!-- http://www.semanticweb.org/paulagranadosgarcia/CuCoO/hasConventus -->

    <owl:ObjectProperty rdf:about="http://www.semanticweb.org/paulagranadosgarcia/CuCoO/hasConventus">
        <rdfs:subPropertyOf rdf:resource="http://www.semanticweb.org/paulagranadosgarcia/CuCoO/hasAdministrativeOrganisation"/>
        <rdfs:domain rdf:resource="http://www.semanticweb.org/paulagranadosgarcia/CuCoO/Settlement"/>
        <rdfs:range rdf:resource="http://www.semanticweb.org/paulagranadosgarcia/CuCoO/Conventus"/>
        <rdfs:comment>relates a settlement (e.g. Gades) with the conventus it belonged to (e.g. Conventus Gaditanus).</rdfs:comment>
    </owl:ObjectProperty>
    


    <!-- http://www.semanticweb.org/paulagranadosgarcia/CuCoO/hasEthnicIdentity -->

    <owl:ObjectProperty rdf:about="http://www.semanticweb.org/paulagranadosgarcia/CuCoO/hasEthnicIdentity">
        <rdfs:domain rdf:resource="http://www.semanticweb.org/paulagranadosgarcia/CuCoO/Person"/>
        <rdfs:range rdf:resource="http://www.semanticweb.org/paulagranadosgarcia/CuCoO/EthnicIdentity"/>
    </owl:ObjectProperty>
    


    <!-- http://www.semanticweb.org/paulagranadosgarcia/CuCoO/hasGenderIdentity -->

    <owl:ObjectProperty rdf:about="http://www.semanticweb.org/paulagranadosgarcia/CuCoO/hasGenderIdentity">
        <rdfs:domain rdf:resource="http://www.semanticweb.org/paulagranadosgarcia/CuCoO/Person"/>
        <rdfs:range rdf:resource="http://www.semanticweb.org/paulagranadosgarcia/CuCoO/GenderIdentity"/>
    </owl:ObjectProperty>
    


    <!-- http://www.semanticweb.org/paulagranadosgarcia/CuCoO/hasIconography -->

    <owl:ObjectProperty rdf:about="http://www.semanticweb.org/paulagranadosgarcia/CuCoO/hasIconography">
        <rdfs:subPropertyOf rdf:resource="http://www.semanticweb.org/paulagranadosgarcia/CuCoO/hasTrait"/>
        <rdfs:domain rdf:resource="http://www.semanticweb.org/paulagranadosgarcia/CuCoO/Thing"/>
        <rdfs:range rdf:resource="http://www.semanticweb.org/paulagranadosgarcia/CuCoO/Iconography"/>
        <rdfs:comment>Relates a sculpture, a coin or a EpigraphicInscription with the iconography that it displays.</rdfs:comment>
    </owl:ObjectProperty>
    


    <!-- http://www.semanticweb.org/paulagranadosgarcia/CuCoO/hasLanguage -->

    <owl:ObjectProperty rdf:about="http://www.semanticweb.org/paulagranadosgarcia/CuCoO/hasLanguage">
        <rdfs:subPropertyOf rdf:resource="http://www.semanticweb.org/paulagranadosgarcia/CuCoO/hasTrait"/>
        <rdfs:domain rdf:resource="http://www.semanticweb.org/paulagranadosgarcia/CuCoO/Text"/>
        <rdfs:comment>Relates a text with the language it displays.</rdfs:comment>
    </owl:ObjectProperty>
    


    <!-- http://www.semanticweb.org/paulagranadosgarcia/CuCoO/hasMaterial -->

    <owl:ObjectProperty rdf:about="http://www.semanticweb.org/paulagranadosgarcia/CuCoO/hasMaterial">
        <rdfs:subPropertyOf rdf:resource="http://www.semanticweb.org/paulagranadosgarcia/CuCoO/hasTrait"/>
        <rdfs:domain rdf:resource="http://www.semanticweb.org/paulagranadosgarcia/CuCoO/Thing"/>
        <rdfs:range rdf:resource="http://www.semanticweb.org/paulagranadosgarcia/CuCoO/Material"/>
        <rdfs:comment>Relates epigraphicinscription, coin and sculpture to the material they are made of.</rdfs:comment>
    </owl:ObjectProperty>
    


    <!-- http://www.semanticweb.org/paulagranadosgarcia/CuCoO/hasMeasure -->

    <owl:ObjectProperty rdf:about="http://www.semanticweb.org/paulagranadosgarcia/CuCoO/hasMeasure">
        <rdfs:subPropertyOf rdf:resource="http://www.semanticweb.org/paulagranadosgarcia/CuCoO/hasTrait"/>
        <rdfs:domain rdf:resource="http://www.semanticweb.org/paulagranadosgarcia/CuCoO/Thing"/>
        <rdfs:range rdf:resource="http://www.semanticweb.org/paulagranadosgarcia/CuCoO/Measure"/>
        <rdfs:comment>Relates sculpture, coin and epigraphicinscription to their measures.</rdfs:comment>
    </owl:ObjectProperty>
    


    <!-- http://www.semanticweb.org/paulagranadosgarcia/CuCoO/hasMetrology -->

    <owl:ObjectProperty rdf:about="http://www.semanticweb.org/paulagranadosgarcia/CuCoO/hasMetrology">
        <rdfs:subPropertyOf rdf:resource="http://www.semanticweb.org/paulagranadosgarcia/CuCoO/hasTrait"/>
        <rdfs:domain rdf:resource="http://www.semanticweb.org/paulagranadosgarcia/CuCoO/Coin"/>
        <rdfs:comment>Relates a mint with its metrology.</rdfs:comment>
    </owl:ObjectProperty>
    


    <!-- http://www.semanticweb.org/paulagranadosgarcia/CuCoO/hasProvince -->

    <owl:ObjectProperty rdf:about="http://www.semanticweb.org/paulagranadosgarcia/CuCoO/hasProvince">
        <rdfs:subPropertyOf rdf:resource="http://www.semanticweb.org/paulagranadosgarcia/CuCoO/hasAdministrativeOrganisation"/>
        <rdfs:domain rdf:resource="http://www.semanticweb.org/paulagranadosgarcia/CuCoO/Conventus"/>
        <rdfs:domain rdf:resource="http://www.semanticweb.org/paulagranadosgarcia/CuCoO/Settlement"/>
        <rdfs:range rdf:resource="http://www.semanticweb.org/paulagranadosgarcia/CuCoO/Province"/>
        <rdfs:comment>Relates a settlement to the province it belonged to.</rdfs:comment>
    </owl:ObjectProperty>
    


    <!-- http://www.semanticweb.org/paulagranadosgarcia/CuCoO/hasRelationship -->

    <owl:ObjectProperty rdf:about="http://www.semanticweb.org/paulagranadosgarcia/CuCoO/hasRelationship">
        <rdfs:domain rdf:resource="http://www.semanticweb.org/paulagranadosgarcia/CuCoO/CulturalContactAgent"/>
        <rdfs:range rdf:resource="http://www.semanticweb.org/paulagranadosgarcia/CuCoO/CulturalContactRelationship"/>
        <rdfs:comment>It relates a cultural contact recipient to the kind of cultural contact relationship it is related to.</rdfs:comment>
    </owl:ObjectProperty>
    


    <!-- http://www.semanticweb.org/paulagranadosgarcia/CuCoO/hasReligiousIdentity -->

    <owl:ObjectProperty rdf:about="http://www.semanticweb.org/paulagranadosgarcia/CuCoO/hasReligiousIdentity">
        <rdfs:domain rdf:resource="http://www.semanticweb.org/paulagranadosgarcia/CuCoO/Person"/>
        <rdfs:range rdf:resource="http://www.semanticweb.org/paulagranadosgarcia/CuCoO/ReligiousIdentity"/>
    </owl:ObjectProperty>
    


    <!-- http://www.semanticweb.org/paulagranadosgarcia/CuCoO/hasSettlementLegalStatus -->

    <owl:ObjectProperty rdf:about="http://www.semanticweb.org/paulagranadosgarcia/CuCoO/hasSettlementLegalStatus">
        <rdfs:subPropertyOf rdf:resource="http://www.semanticweb.org/paulagranadosgarcia/CuCoO/hasTrait"/>
        <rdfs:domain rdf:resource="http://www.semanticweb.org/paulagranadosgarcia/CuCoO/Settlement"/>
        <rdfs:range rdf:resource="http://www.semanticweb.org/paulagranadosgarcia/CuCoO/SettlementLegalStatus"/>
        <rdfs:comment>Relates a settlement with the legal status it recived under Roman adiministration.</rdfs:comment>
    </owl:ObjectProperty>
    


    <!-- http://www.semanticweb.org/paulagranadosgarcia/CuCoO/hasSocialIdentity -->

    <owl:ObjectProperty rdf:about="http://www.semanticweb.org/paulagranadosgarcia/CuCoO/hasSocialIdentity">
        <rdfs:domain rdf:resource="http://www.semanticweb.org/paulagranadosgarcia/CuCoO/Person"/>
        <rdfs:range rdf:resource="http://www.semanticweb.org/paulagranadosgarcia/CuCoO/SocialIdentity"/>
    </owl:ObjectProperty>
    


    <!-- http://www.semanticweb.org/paulagranadosgarcia/CuCoO/hasText -->

    <owl:ObjectProperty rdf:about="http://www.semanticweb.org/paulagranadosgarcia/CuCoO/hasText">
        <rdfs:subPropertyOf rdf:resource="http://www.semanticweb.org/paulagranadosgarcia/CuCoO/hasTrait"/>
        <rdfs:domain rdf:resource="http://www.semanticweb.org/paulagranadosgarcia/CuCoO/Thing"/>
        <rdfs:range rdf:resource="http://www.semanticweb.org/paulagranadosgarcia/CuCoO/Text"/>
        <rdfs:comment>Relates an epigraphic inscription or a coin with the text it displays.</rdfs:comment>
    </owl:ObjectProperty>
    


    <!-- http://www.semanticweb.org/paulagranadosgarcia/CuCoO/hasTrait -->

    <owl:ObjectProperty rdf:about="http://www.semanticweb.org/paulagranadosgarcia/CuCoO/hasTrait">
        <rdfs:domain rdf:resource="http://www.semanticweb.org/paulagranadosgarcia/CuCoO/CulturalContactAgent"/>
        <rdfs:range rdf:resource="http://www.semanticweb.org/paulagranadosgarcia/CuCoO/CulturalContactTrait"/>
        <rdfs:comment>Relates a CulturalContactRecipient with the CultursalTrait it displays.</rdfs:comment>
    </owl:ObjectProperty>
    


    <!-- http://www.semanticweb.org/paulagranadosgarcia/CuCoO/isAssociatedWith -->

    <owl:ObjectProperty rdf:about="http://www.semanticweb.org/paulagranadosgarcia/CuCoO/isAssociatedWith">
        <rdfs:domain rdf:resource="http://www.semanticweb.org/paulagranadosgarcia/CuCoO/CulturalContactAgent"/>
        <rdfs:domain rdf:resource="http://www.semanticweb.org/paulagranadosgarcia/CuCoO/CulturalContactTrait"/>
        <rdfs:range rdf:resource="http://www.semanticweb.org/paulagranadosgarcia/CuCoO/CulturalIdentity"/>
        <rdfs:comment>Associates a CulturalContactTrait with a cultural identity.</rdfs:comment>
    </owl:ObjectProperty>
    


    <!-- 
    ///////////////////////////////////////////////////////////////////////////////////////
    //
    // Classes
    //
    ///////////////////////////////////////////////////////////////////////////////////////
     -->

    


    <!-- http://www.semanticweb.org/paulagranadosgarcia/CuCoO/Accesories -->

    <owl:Class rdf:about="http://www.semanticweb.org/paulagranadosgarcia/CuCoO/Accesories">
        <rdfs:subClassOf rdf:resource="http://www.semanticweb.org/paulagranadosgarcia/CuCoO/PhysicalAppearance"/>
    </owl:Class>
    


    <!-- http://www.semanticweb.org/paulagranadosgarcia/CuCoO/Carving -->

    <owl:Class rdf:about="http://www.semanticweb.org/paulagranadosgarcia/CuCoO/Carving">
        <rdfs:subClassOf rdf:resource="http://www.semanticweb.org/paulagranadosgarcia/CuCoO/CulturalContactTrait"/>
    </owl:Class>
    


    <!-- http://www.semanticweb.org/paulagranadosgarcia/CuCoO/Civitas -->

    <owl:Class rdf:about="http://www.semanticweb.org/paulagranadosgarcia/CuCoO/Civitas">
        <rdfs:subClassOf rdf:resource="http://www.semanticweb.org/paulagranadosgarcia/CuCoO/SettlementLegalStatus"/>
        <rdfs:comment>Most inferior legal status granted to a settlment.</rdfs:comment>
    </owl:Class>
    


    <!-- http://www.semanticweb.org/paulagranadosgarcia/CuCoO/Clothes -->

    <owl:Class rdf:about="http://www.semanticweb.org/paulagranadosgarcia/CuCoO/Clothes">
        <rdfs:subClassOf rdf:resource="http://www.semanticweb.org/paulagranadosgarcia/CuCoO/PhysicalAppearance"/>
    </owl:Class>
    


    <!-- http://www.semanticweb.org/paulagranadosgarcia/CuCoO/Coin -->

    <owl:Class rdf:about="http://www.semanticweb.org/paulagranadosgarcia/CuCoO/Coin">
        <rdfs:subClassOf rdf:resource="http://www.semanticweb.org/paulagranadosgarcia/CuCoO/Thing"/>
    </owl:Class>
    


    <!-- http://www.semanticweb.org/paulagranadosgarcia/CuCoO/Colonia -->

    <owl:Class rdf:about="http://www.semanticweb.org/paulagranadosgarcia/CuCoO/Colonia">
        <rdfs:subClassOf rdf:resource="http://www.semanticweb.org/paulagranadosgarcia/CuCoO/SettlementLegalStatus"/>
        <rdfs:comment>City founded ex-novo by Roman colonisers or maximum legal status granted to a settlement.</rdfs:comment>
    </owl:Class>
    


    <!-- http://www.semanticweb.org/paulagranadosgarcia/CuCoO/Conquest -->

    <owl:Class rdf:about="http://www.semanticweb.org/paulagranadosgarcia/CuCoO/Conquest">
        <rdfs:subClassOf rdf:resource="http://www.semanticweb.org/paulagranadosgarcia/CuCoO/CulturalContactContext"/>
        <rdfs:comment>The cultural contact situation happens during a process of colonial conquest (e.g. Roman colonisation of the Iberian Penisula).</rdfs:comment>
    </owl:Class>
    


    <!-- http://www.semanticweb.org/paulagranadosgarcia/CuCoO/Conventus -->

    <owl:Class rdf:about="http://www.semanticweb.org/paulagranadosgarcia/CuCoO/Conventus">
        <rdfs:subClassOf rdf:resource="http://www.semanticweb.org/paulagranadosgarcia/CuCoO/SettlementAdministrativeOrganisation"/>
        <rdfs:comment>Roman administrative entitiy of control over the territory, smaller than a province, that referred to the assembly of communities of indigenous and Roman citizens.</rdfs:comment>
    </owl:Class>
    


    <!-- http://www.semanticweb.org/paulagranadosgarcia/CuCoO/CulturalContact -->

    <owl:Class rdf:about="http://www.semanticweb.org/paulagranadosgarcia/CuCoO/CulturalContact">
        <rdfs:subClassOf rdf:resource="http://www.semanticweb.org/paulagranadosgarcia/CuCoO/Entitiy"/>
        <rdfs:comment>Refers to the phenomenon of interaction amongst at least two communities with different cultural and ethnical backgrounds.</rdfs:comment>
    </owl:Class>
    


    <!-- http://www.semanticweb.org/paulagranadosgarcia/CuCoO/CulturalContactAgent -->

    <owl:Class rdf:about="http://www.semanticweb.org/paulagranadosgarcia/CuCoO/CulturalContactAgent">
        <rdfs:subClassOf rdf:resource="http://www.semanticweb.org/paulagranadosgarcia/CuCoO/Entitiy"/>
        <rdfs:comment>Refers to things or people that embody cultural contact meaning.</rdfs:comment>
    </owl:Class>
    


    <!-- http://www.semanticweb.org/paulagranadosgarcia/CuCoO/CulturalContactAspects -->

    <owl:Class rdf:about="http://www.semanticweb.org/paulagranadosgarcia/CuCoO/CulturalContactAspects">
        <rdfs:subClassOf rdf:resource="http://www.semanticweb.org/paulagranadosgarcia/CuCoO/CulturalContactFeature"/>
        <rdfs:comment></rdfs:comment>
        <rdfs:comment>Character of the cultural contact situation (e.g. Economic, the evidence can proove the establishment of some economic relationship amongst the different comunities involved in the situation of cultural contact).</rdfs:comment>
    </owl:Class>
    


    <!-- http://www.semanticweb.org/paulagranadosgarcia/CuCoO/CulturalContactContext -->

    <owl:Class rdf:about="http://www.semanticweb.org/paulagranadosgarcia/CuCoO/CulturalContactContext">
        <rdfs:subClassOf rdf:resource="http://www.semanticweb.org/paulagranadosgarcia/CuCoO/CulturalContactFeature"/>
        <rdfs:comment>Refers to the context in which the situation of cultural contact takes place (e.g. in a context of trade, the main objective behind the cultural contact is economic profit).</rdfs:comment>
    </owl:Class>
    


    <!-- http://www.semanticweb.org/paulagranadosgarcia/CuCoO/CulturalContactFeature -->

    <owl:Class rdf:about="http://www.semanticweb.org/paulagranadosgarcia/CuCoO/CulturalContactFeature">
        <rdfs:subClassOf rdf:resource="http://www.semanticweb.org/paulagranadosgarcia/CuCoO/Entitiy"/>
        <rdfs:comment>Refers to any cultural contact feature that can be identified in the entities. For example, cultural contact traits or cultural contact aspects.</rdfs:comment>
    </owl:Class>
    


    <!-- http://www.semanticweb.org/paulagranadosgarcia/CuCoO/CulturalContactRelationship -->

    <owl:Class rdf:about="http://www.semanticweb.org/paulagranadosgarcia/CuCoO/CulturalContactRelationship">
        <rdfs:subClassOf rdf:resource="http://www.semanticweb.org/paulagranadosgarcia/CuCoO/CulturalContactFeature"/>
        <rdfs:comment>Relationship established amongst the different groups involved in the cultural contact situation.</rdfs:comment>
    </owl:Class>
    


    <!-- http://www.semanticweb.org/paulagranadosgarcia/CuCoO/CulturalContactTrait -->

    <owl:Class rdf:about="http://www.semanticweb.org/paulagranadosgarcia/CuCoO/CulturalContactTrait">
        <rdfs:subClassOf rdf:resource="http://www.semanticweb.org/paulagranadosgarcia/CuCoO/CulturalContactFeature"/>
        <rdfs:comment>Characteristic of human action accquired and transmited by any kind of communication in a situation of cultural contact.</rdfs:comment>
    </owl:Class>
    


    <!-- http://www.semanticweb.org/paulagranadosgarcia/CuCoO/CulturalIdentity -->

    <owl:Class rdf:about="http://www.semanticweb.org/paulagranadosgarcia/CuCoO/CulturalIdentity">
        <rdfs:subClassOf rdf:resource="http://www.semanticweb.org/paulagranadosgarcia/CuCoO/Entitiy"/>
        <rdfs:comment>Self-conscious association of a group or a person with a culturally constructed group identitiy that intersect with others in the identification of, and interaction, between groups.Refers to the elements that constitue a person cultural identity.</rdfs:comment>
    </owl:Class>
    


    <!-- http://www.semanticweb.org/paulagranadosgarcia/CuCoO/Economic -->

    <owl:Class rdf:about="http://www.semanticweb.org/paulagranadosgarcia/CuCoO/Economic">
        <rdfs:subClassOf rdf:resource="http://www.semanticweb.org/paulagranadosgarcia/CuCoO/CulturalContactAspects"/>
        <rdfs:comment>An economic relationship amongst the different culutral groups can be demonstrated in the evidence (e.g. coins distribution).</rdfs:comment>
    </owl:Class>
    


    <!-- http://www.semanticweb.org/paulagranadosgarcia/CuCoO/Entitiy -->

    <owl:Class rdf:about="http://www.semanticweb.org/paulagranadosgarcia/CuCoO/Entitiy"/>
    


    <!-- http://www.semanticweb.org/paulagranadosgarcia/CuCoO/EpigraphicInscription -->

    <owl:Class rdf:about="http://www.semanticweb.org/paulagranadosgarcia/CuCoO/EpigraphicInscription">
        <rdfs:subClassOf rdf:resource="http://www.semanticweb.org/paulagranadosgarcia/CuCoO/Thing"/>
    </owl:Class>
    


    <!-- http://www.semanticweb.org/paulagranadosgarcia/CuCoO/Equal -->

    <owl:Class rdf:about="http://www.semanticweb.org/paulagranadosgarcia/CuCoO/Equal">
        <rdfs:subClassOf rdf:resource="http://www.semanticweb.org/paulagranadosgarcia/CuCoO/CulturalContactRelationship"/>
        <owl:disjointWith rdf:resource="http://www.semanticweb.org/paulagranadosgarcia/CuCoO/Unequal"/>
        <rdfs:comment>Relationship in which all groups involved in the cultural contact situation are at the same level.</rdfs:comment>
    </owl:Class>
    


    <!-- http://www.semanticweb.org/paulagranadosgarcia/CuCoO/EthnicIdentity -->

    <owl:Class rdf:about="http://www.semanticweb.org/paulagranadosgarcia/CuCoO/EthnicIdentity">
        <rdfs:subClassOf rdf:resource="http://www.semanticweb.org/paulagranadosgarcia/CuCoO/CulturalIdentity"/>
        <rdfs:comment>Refers to the &apos;self-conscious identification of a person or a group with a series of cultural traits, plus notions of shared history shared territory, kinship and common descent which differentiate it from other groups&apos;.</rdfs:comment>
    </owl:Class>
    


    <!-- http://www.semanticweb.org/paulagranadosgarcia/CuCoO/GenderIdentity -->

    <owl:Class rdf:about="http://www.semanticweb.org/paulagranadosgarcia/CuCoO/GenderIdentity">
        <rdfs:subClassOf rdf:resource="http://www.semanticweb.org/paulagranadosgarcia/CuCoO/CulturalIdentity"/>
        <rdfs:comment>that aspect of a person conceptualization wich results from identification with a gender.</rdfs:comment>
    </owl:Class>
    


    <!-- http://www.semanticweb.org/paulagranadosgarcia/CuCoO/Hairstyle -->

    <owl:Class rdf:about="http://www.semanticweb.org/paulagranadosgarcia/CuCoO/Hairstyle">
        <rdfs:subClassOf rdf:resource="http://www.semanticweb.org/paulagranadosgarcia/CuCoO/PhysicalAppearance"/>
    </owl:Class>
    


    <!-- http://www.semanticweb.org/paulagranadosgarcia/CuCoO/Iconography -->

    <owl:Class rdf:about="http://www.semanticweb.org/paulagranadosgarcia/CuCoO/Iconography">
        <rdfs:subClassOf rdf:resource="http://www.semanticweb.org/paulagranadosgarcia/CuCoO/CulturalContactTrait"/>
    </owl:Class>
    


    <!-- http://www.semanticweb.org/paulagranadosgarcia/CuCoO/ImpermeableCulturalContact -->

    <owl:Class rdf:about="http://www.semanticweb.org/paulagranadosgarcia/CuCoO/ImpermeableCulturalContact">
        <rdfs:subClassOf rdf:resource="http://www.semanticweb.org/paulagranadosgarcia/CuCoO/CulturalContact"/>
        <owl:disjointWith rdf:resource="http://www.semanticweb.org/paulagranadosgarcia/CuCoO/PermeableCulturalContact"/>
        <rdfs:comment>Situation of cultural contact (e.g. Roman foundation of a colonia) where there is no evidence for cultural influence (e.g. no appearance of indigenous influences in the material culture).</rdfs:comment>
    </owl:Class>
    


    <!-- http://www.semanticweb.org/paulagranadosgarcia/CuCoO/Linguistic -->

    <owl:Class rdf:about="http://www.semanticweb.org/paulagranadosgarcia/CuCoO/Linguistic">
        <rdfs:subClassOf rdf:resource="http://www.semanticweb.org/paulagranadosgarcia/CuCoO/CulturalContactAspects"/>
        <rdfs:comment>Linguistic influence amongst the different cultural groups can be demonstrated int he evidence (e.g. bilingual inscriptions or use of foreign alphabets to record indigenous onomastica).</rdfs:comment>
    </owl:Class>
    


    <!-- http://www.semanticweb.org/paulagranadosgarcia/CuCoO/Material -->

    <owl:Class rdf:about="http://www.semanticweb.org/paulagranadosgarcia/CuCoO/Material">
        <rdfs:subClassOf rdf:resource="http://www.semanticweb.org/paulagranadosgarcia/CuCoO/CulturalContactTrait"/>
    </owl:Class>
    


    <!-- http://www.semanticweb.org/paulagranadosgarcia/CuCoO/Measure -->

    <owl:Class rdf:about="http://www.semanticweb.org/paulagranadosgarcia/CuCoO/Measure">
        <rdfs:subClassOf rdf:resource="http://www.semanticweb.org/paulagranadosgarcia/CuCoO/CulturalContactTrait"/>
    </owl:Class>
    


    <!-- http://www.semanticweb.org/paulagranadosgarcia/CuCoO/Migration -->

    <owl:Class rdf:about="http://www.semanticweb.org/paulagranadosgarcia/CuCoO/Migration">
        <rdfs:subClassOf rdf:resource="http://www.semanticweb.org/paulagranadosgarcia/CuCoO/CulturalContactContext"/>
        <rdfs:comment>The cultural contact situation happens during a process of migration.</rdfs:comment>
    </owl:Class>
    


    <!-- http://www.semanticweb.org/paulagranadosgarcia/CuCoO/Municipium -->

    <owl:Class rdf:about="http://www.semanticweb.org/paulagranadosgarcia/CuCoO/Municipium">
        <rdfs:subClassOf rdf:resource="http://www.semanticweb.org/paulagranadosgarcia/CuCoO/SettlementLegalStatus"/>
        <rdfs:comment>City-states with walls brought into the city-state of Rome and under the Roman jurisdiction but remaining independent in some aspects.</rdfs:comment>
    </owl:Class>
    


    <!-- http://www.semanticweb.org/paulagranadosgarcia/CuCoO/PermeableCulturalContact -->

    <owl:Class rdf:about="http://www.semanticweb.org/paulagranadosgarcia/CuCoO/PermeableCulturalContact">
        <rdfs:subClassOf rdf:resource="http://www.semanticweb.org/paulagranadosgarcia/CuCoO/CulturalContact"/>
        <rdfs:comment>Situation of cultural contact (e.g. Roman conquest of the Iberian Peninsula) where there is evidence for cultural influence (e.g. appearance of Roman influences in the material culture).</rdfs:comment>
    </owl:Class>
    


    <!-- http://www.semanticweb.org/paulagranadosgarcia/CuCoO/Person -->

    <owl:Class rdf:about="http://www.semanticweb.org/paulagranadosgarcia/CuCoO/Person">
        <rdfs:subClassOf rdf:resource="http://www.semanticweb.org/paulagranadosgarcia/CuCoO/CulturalContactAgent"/>
    </owl:Class>
    


    <!-- http://www.semanticweb.org/paulagranadosgarcia/CuCoO/PersonLegalStatus -->

    <owl:Class rdf:about="http://www.semanticweb.org/paulagranadosgarcia/CuCoO/PersonLegalStatus">
        <rdfs:subClassOf rdf:resource="http://www.semanticweb.org/paulagranadosgarcia/CuCoO/SocialIdentity"/>
        <rdfs:comment>Person legal status according to Roman law.</rdfs:comment>
    </owl:Class>
    


    <!-- http://www.semanticweb.org/paulagranadosgarcia/CuCoO/PhysicalAppearance -->

    <owl:Class rdf:about="http://www.semanticweb.org/paulagranadosgarcia/CuCoO/PhysicalAppearance">
        <rdfs:subClassOf rdf:resource="http://www.semanticweb.org/paulagranadosgarcia/CuCoO/CulturalContactTrait"/>
        <rdfs:comment>Refers to all things that constitute one personâ€™s appearance.</rdfs:comment>
    </owl:Class>
    


    <!-- http://www.semanticweb.org/paulagranadosgarcia/CuCoO/Posture -->

    <owl:Class rdf:about="http://www.semanticweb.org/paulagranadosgarcia/CuCoO/Posture">
        <rdfs:subClassOf rdf:resource="http://www.semanticweb.org/paulagranadosgarcia/CuCoO/PhysicalAppearance"/>
    </owl:Class>
    


    <!-- http://www.semanticweb.org/paulagranadosgarcia/CuCoO/Province -->

    <owl:Class rdf:about="http://www.semanticweb.org/paulagranadosgarcia/CuCoO/Province">
        <rdfs:subClassOf rdf:resource="http://www.semanticweb.org/paulagranadosgarcia/CuCoO/SettlementAdministrativeOrganisation"/>
        <rdfs:comment>Roman territorial administrative demarcation of the territory.</rdfs:comment>
    </owl:Class>
    


    <!-- http://www.semanticweb.org/paulagranadosgarcia/CuCoO/Religious -->

    <owl:Class rdf:about="http://www.semanticweb.org/paulagranadosgarcia/CuCoO/Religious">
        <rdfs:subClassOf rdf:resource="http://www.semanticweb.org/paulagranadosgarcia/CuCoO/CulturalContactAspects"/>
        <rdfs:comment>An exchange of religous influences amongst the different cultural groups can be demonstrated in the evidence (e.g. syncretism between local and foreign deities).</rdfs:comment>
    </owl:Class>
    


    <!-- http://www.semanticweb.org/paulagranadosgarcia/CuCoO/ReligiousIdentity -->

    <owl:Class rdf:about="http://www.semanticweb.org/paulagranadosgarcia/CuCoO/ReligiousIdentity">
        <rdfs:subClassOf rdf:resource="http://www.semanticweb.org/paulagranadosgarcia/CuCoO/CulturalIdentity"/>
        <rdfs:comment>Refers to a person or a gruop believes and practices.</rdfs:comment>
    </owl:Class>
    


    <!-- http://www.semanticweb.org/paulagranadosgarcia/CuCoO/Sculpture -->

    <owl:Class rdf:about="http://www.semanticweb.org/paulagranadosgarcia/CuCoO/Sculpture">
        <rdfs:subClassOf rdf:resource="http://www.semanticweb.org/paulagranadosgarcia/CuCoO/Thing"/>
    </owl:Class>
    


    <!-- http://www.semanticweb.org/paulagranadosgarcia/CuCoO/Settlement -->

    <owl:Class rdf:about="http://www.semanticweb.org/paulagranadosgarcia/CuCoO/Settlement">
        <rdfs:subClassOf rdf:resource="http://www.semanticweb.org/paulagranadosgarcia/CuCoO/CulturalContactAgent"/>
    </owl:Class>
    


    <!-- http://www.semanticweb.org/paulagranadosgarcia/CuCoO/SettlementAdministrativeOrganisation -->

    <owl:Class rdf:about="http://www.semanticweb.org/paulagranadosgarcia/CuCoO/SettlementAdministrativeOrganisation">
        <rdfs:subClassOf rdf:resource="http://www.semanticweb.org/paulagranadosgarcia/CuCoO/CulturalContactTrait"/>
    </owl:Class>
    


    <!-- http://www.semanticweb.org/paulagranadosgarcia/CuCoO/SettlementLegalStatus -->

    <owl:Class rdf:about="http://www.semanticweb.org/paulagranadosgarcia/CuCoO/SettlementLegalStatus">
        <rdfs:subClassOf rdf:resource="http://www.semanticweb.org/paulagranadosgarcia/CuCoO/CulturalContactTrait"/>
        <rdfs:comment>City legal status according to Roman law.</rdfs:comment>
    </owl:Class>
    


    <!-- http://www.semanticweb.org/paulagranadosgarcia/CuCoO/Social -->

    <owl:Class rdf:about="http://www.semanticweb.org/paulagranadosgarcia/CuCoO/Social">
        <rdfs:subClassOf rdf:resource="http://www.semanticweb.org/paulagranadosgarcia/CuCoO/CulturalContactAspects"/>
        <rdfs:comment>The evidence demonstrates exchange of social behaviours amongst the different cultural groups involved in the cultural contact situation (e.g. changes in the construction habits).</rdfs:comment>
    </owl:Class>
    


    <!-- http://www.semanticweb.org/paulagranadosgarcia/CuCoO/SocialIdentity -->

    <owl:Class rdf:about="http://www.semanticweb.org/paulagranadosgarcia/CuCoO/SocialIdentity">
        <rdfs:subClassOf rdf:resource="http://www.semanticweb.org/paulagranadosgarcia/CuCoO/CulturalIdentity"/>
        <rdfs:comment>that aspect of a person conceptualization associated with its role in society.</rdfs:comment>
    </owl:Class>
    


    <!-- http://www.semanticweb.org/paulagranadosgarcia/CuCoO/Style -->

    <owl:Class rdf:about="http://www.semanticweb.org/paulagranadosgarcia/CuCoO/Style">
        <rdfs:subClassOf rdf:resource="http://www.semanticweb.org/paulagranadosgarcia/CuCoO/CulturalContactTrait"/>
    </owl:Class>
    


    <!-- http://www.semanticweb.org/paulagranadosgarcia/CuCoO/Text -->

    <owl:Class rdf:about="http://www.semanticweb.org/paulagranadosgarcia/CuCoO/Text">
        <rdfs:subClassOf rdf:resource="http://www.semanticweb.org/paulagranadosgarcia/CuCoO/CulturalContactTrait"/>
    </owl:Class>
    


    <!-- http://www.semanticweb.org/paulagranadosgarcia/CuCoO/Thing -->

    <owl:Class rdf:about="http://www.semanticweb.org/paulagranadosgarcia/CuCoO/Thing">
        <rdfs:subClassOf rdf:resource="http://www.semanticweb.org/paulagranadosgarcia/CuCoO/CulturalContactAgent"/>
    </owl:Class>
    


    <!-- http://www.semanticweb.org/paulagranadosgarcia/CuCoO/Trade -->

    <owl:Class rdf:about="http://www.semanticweb.org/paulagranadosgarcia/CuCoO/Trade">
        <rdfs:subClassOf rdf:resource="http://www.semanticweb.org/paulagranadosgarcia/CuCoO/CulturalContactContext"/>
        <rdfs:comment>The cultural contact situation happens during a process of trade (e.g. Phoenician and Greek settlements in the peninsula).</rdfs:comment>
    </owl:Class>
    


    <!-- http://www.semanticweb.org/paulagranadosgarcia/CuCoO/Unequal -->

    <owl:Class rdf:about="http://www.semanticweb.org/paulagranadosgarcia/CuCoO/Unequal">
        <rdfs:subClassOf rdf:resource="http://www.semanticweb.org/paulagranadosgarcia/CuCoO/CulturalContactRelationship"/>
        <rdfs:comment>Relationship in which the groups involved are in different  levels (e.g. one group is under the control of other group).</rdfs:comment>
    </owl:Class>
    


    <!-- http://www.semanticweb.org/paulagranadosgarcia/CuCoO/War -->

    <owl:Class rdf:about="http://www.semanticweb.org/paulagranadosgarcia/CuCoO/War">
        <rdfs:subClassOf rdf:resource="http://www.semanticweb.org/paulagranadosgarcia/CuCoO/CulturalContactContext"/>
        <rdfs:comment>The cultural contact situation happens during a process of armed conflict (e.g. Punic settlements in Iberia).</rdfs:comment>
    </owl:Class>
    


    <!-- http://www.semanticweb.org/paulagranadosgarcia/CuCoO/Weight -->

    <owl:Class rdf:about="http://www.semanticweb.org/paulagranadosgarcia/CuCoO/Weight">
        <rdfs:subClassOf rdf:resource="http://www.semanticweb.org/paulagranadosgarcia/CuCoO/CulturalContactTrait"/>
    </owl:Class>
    


    <!-- 
    ///////////////////////////////////////////////////////////////////////////////////////
    //
    // Individuals
    //
    ///////////////////////////////////////////////////////////////////////////////////////
     -->

    


    <!-- http://www.semanticweb.org/paulagranadosgarcia/CuCoO/Architecture -->

    <owl:NamedIndividual rdf:about="http://www.semanticweb.org/paulagranadosgarcia/CuCoO/Architecture">
        <rdf:type rdf:resource="http://www.semanticweb.org/paulagranadosgarcia/CuCoO/Measure"/>
    </owl:NamedIndividual>
    


    <!-- http://www.semanticweb.org/paulagranadosgarcia/CuCoO/Astigitanus -->

    <owl:NamedIndividual rdf:about="http://www.semanticweb.org/paulagranadosgarcia/CuCoO/Astigitanus">
        <rdf:type rdf:resource="http://www.semanticweb.org/paulagranadosgarcia/CuCoO/Conventus"/>
    </owl:NamedIndividual>
    


    <!-- http://www.semanticweb.org/paulagranadosgarcia/CuCoO/Bastetani -->

    <owl:NamedIndividual rdf:about="http://www.semanticweb.org/paulagranadosgarcia/CuCoO/Bastetani">
        <rdf:type rdf:resource="http://www.semanticweb.org/paulagranadosgarcia/CuCoO/EthnicIdentity"/>
    </owl:NamedIndividual>
    


    <!-- http://www.semanticweb.org/paulagranadosgarcia/CuCoO/Carving -->

    <owl:NamedIndividual rdf:about="http://www.semanticweb.org/paulagranadosgarcia/CuCoO/Carving"/>
    


    <!-- http://www.semanticweb.org/paulagranadosgarcia/CuCoO/City -->

    <owl:NamedIndividual rdf:about="http://www.semanticweb.org/paulagranadosgarcia/CuCoO/City"/>
    


    <!-- http://www.semanticweb.org/paulagranadosgarcia/CuCoO/Coinage -->

    <owl:NamedIndividual rdf:about="http://www.semanticweb.org/paulagranadosgarcia/CuCoO/Coinage">
        <rdf:type rdf:resource="http://www.semanticweb.org/paulagranadosgarcia/CuCoO/CulturalContactAgent"/>
    </owl:NamedIndividual>
    


    <!-- http://www.semanticweb.org/paulagranadosgarcia/CuCoO/Cordubensis -->

    <owl:NamedIndividual rdf:about="http://www.semanticweb.org/paulagranadosgarcia/CuCoO/Cordubensis">
        <rdf:type rdf:resource="http://www.semanticweb.org/paulagranadosgarcia/CuCoO/Conventus"/>
    </owl:NamedIndividual>
    


    <!-- http://www.semanticweb.org/paulagranadosgarcia/CuCoO/Dress -->

    <owl:NamedIndividual rdf:about="http://www.semanticweb.org/paulagranadosgarcia/CuCoO/Dress">
        <rdf:type rdf:resource="http://www.semanticweb.org/paulagranadosgarcia/CuCoO/Style"/>
    </owl:NamedIndividual>
    


    <!-- http://www.semanticweb.org/paulagranadosgarcia/CuCoO/Epigraphy -->

    <owl:NamedIndividual rdf:about="http://www.semanticweb.org/paulagranadosgarcia/CuCoO/Epigraphy">
        <rdf:type rdf:resource="http://www.semanticweb.org/paulagranadosgarcia/CuCoO/CulturalContactAgent"/>
    </owl:NamedIndividual>
    


    <!-- http://www.semanticweb.org/paulagranadosgarcia/CuCoO/Factory -->

    <owl:NamedIndividual rdf:about="http://www.semanticweb.org/paulagranadosgarcia/CuCoO/Factory"/>
    


    <!-- http://www.semanticweb.org/paulagranadosgarcia/CuCoO/Female -->

    <owl:NamedIndividual rdf:about="http://www.semanticweb.org/paulagranadosgarcia/CuCoO/Female">
        <rdf:type rdf:resource="http://www.semanticweb.org/paulagranadosgarcia/CuCoO/GenderIdentity"/>
    </owl:NamedIndividual>
    


    <!-- http://www.semanticweb.org/paulagranadosgarcia/CuCoO/Gaditanus -->

    <owl:NamedIndividual rdf:about="http://www.semanticweb.org/paulagranadosgarcia/CuCoO/Gaditanus">
        <rdf:type rdf:resource="http://www.semanticweb.org/paulagranadosgarcia/CuCoO/Conventus"/>
    </owl:NamedIndividual>
    


    <!-- http://www.semanticweb.org/paulagranadosgarcia/CuCoO/Greek -->

    <owl:NamedIndividual rdf:about="http://www.semanticweb.org/paulagranadosgarcia/CuCoO/Greek">
        <rdf:type rdf:resource="http://www.semanticweb.org/paulagranadosgarcia/CuCoO/EthnicIdentity"/>
    </owl:NamedIndividual>
    


    <!-- http://www.semanticweb.org/paulagranadosgarcia/CuCoO/High_relief -->

    <owl:NamedIndividual rdf:about="http://www.semanticweb.org/paulagranadosgarcia/CuCoO/High_relief">
        <rdf:type rdf:resource="http://www.semanticweb.org/paulagranadosgarcia/CuCoO/Carving"/>
    </owl:NamedIndividual>
    


    <!-- http://www.semanticweb.org/paulagranadosgarcia/CuCoO/Hispalensis -->

    <owl:NamedIndividual rdf:about="http://www.semanticweb.org/paulagranadosgarcia/CuCoO/Hispalensis">
        <rdf:type rdf:resource="http://www.semanticweb.org/paulagranadosgarcia/CuCoO/Conventus"/>
    </owl:NamedIndividual>
    


    <!-- http://www.semanticweb.org/paulagranadosgarcia/CuCoO/Hispania_Baetica -->

    <owl:NamedIndividual rdf:about="http://www.semanticweb.org/paulagranadosgarcia/CuCoO/Hispania_Baetica">
        <rdf:type rdf:resource="http://www.semanticweb.org/paulagranadosgarcia/CuCoO/Province"/>
    </owl:NamedIndividual>
    


    <!-- http://www.semanticweb.org/paulagranadosgarcia/CuCoO/Hispania_Citerior -->

    <owl:NamedIndividual rdf:about="http://www.semanticweb.org/paulagranadosgarcia/CuCoO/Hispania_Citerior">
        <rdf:type rdf:resource="http://www.semanticweb.org/paulagranadosgarcia/CuCoO/Province"/>
    </owl:NamedIndividual>
    


    <!-- http://www.semanticweb.org/paulagranadosgarcia/CuCoO/Hispania_Tarraconensis -->

    <owl:NamedIndividual rdf:about="http://www.semanticweb.org/paulagranadosgarcia/CuCoO/Hispania_Tarraconensis"/>
    


    <!-- http://www.semanticweb.org/paulagranadosgarcia/CuCoO/Hispania_Ulterior -->

    <owl:NamedIndividual rdf:about="http://www.semanticweb.org/paulagranadosgarcia/CuCoO/Hispania_Ulterior">
        <rdf:type rdf:resource="http://www.semanticweb.org/paulagranadosgarcia/CuCoO/Province"/>
    </owl:NamedIndividual>
    


    <!-- http://www.semanticweb.org/paulagranadosgarcia/CuCoO/Iberian -->

    <owl:NamedIndividual rdf:about="http://www.semanticweb.org/paulagranadosgarcia/CuCoO/Iberian">
        <rdf:type rdf:resource="http://www.semanticweb.org/paulagranadosgarcia/CuCoO/EthnicIdentity"/>
        <rdf:type rdf:resource="http://www.semanticweb.org/paulagranadosgarcia/CuCoO/Text"/>
    </owl:NamedIndividual>
    


    <!-- http://www.semanticweb.org/paulagranadosgarcia/CuCoO/Iconography -->

    <owl:NamedIndividual rdf:about="http://www.semanticweb.org/paulagranadosgarcia/CuCoO/Iconography">
        <rdf:type rdf:resource="http://www.semanticweb.org/paulagranadosgarcia/CuCoO/Style"/>
    </owl:NamedIndividual>
    


    <!-- http://www.semanticweb.org/paulagranadosgarcia/CuCoO/Language -->

    <owl:NamedIndividual rdf:about="http://www.semanticweb.org/paulagranadosgarcia/CuCoO/Language"/>
    


    <!-- http://www.semanticweb.org/paulagranadosgarcia/CuCoO/Latin -->

    <owl:NamedIndividual rdf:about="http://www.semanticweb.org/paulagranadosgarcia/CuCoO/Latin">
        <rdf:type rdf:resource="http://www.semanticweb.org/paulagranadosgarcia/CuCoO/Text"/>
    </owl:NamedIndividual>
    


    <!-- http://www.semanticweb.org/paulagranadosgarcia/CuCoO/Legend -->

    <owl:NamedIndividual rdf:about="http://www.semanticweb.org/paulagranadosgarcia/CuCoO/Legend"/>
    


    <!-- http://www.semanticweb.org/paulagranadosgarcia/CuCoO/Low_relief -->

    <owl:NamedIndividual rdf:about="http://www.semanticweb.org/paulagranadosgarcia/CuCoO/Low_relief">
        <rdf:type rdf:resource="http://www.semanticweb.org/paulagranadosgarcia/CuCoO/Carving"/>
    </owl:NamedIndividual>
    


    <!-- http://www.semanticweb.org/paulagranadosgarcia/CuCoO/Male -->

    <owl:NamedIndividual rdf:about="http://www.semanticweb.org/paulagranadosgarcia/CuCoO/Male">
        <rdf:type rdf:resource="http://www.semanticweb.org/paulagranadosgarcia/CuCoO/GenderIdentity"/>
    </owl:NamedIndividual>
    


    <!-- http://www.semanticweb.org/paulagranadosgarcia/CuCoO/Man_Made_Object -->

    <owl:NamedIndividual rdf:about="http://www.semanticweb.org/paulagranadosgarcia/CuCoO/Man_Made_Object">
        <rdf:type rdf:resource="http://www.semanticweb.org/paulagranadosgarcia/CuCoO/CulturalContactAgent"/>
    </owl:NamedIndividual>
    


    <!-- http://www.semanticweb.org/paulagranadosgarcia/CuCoO/Mansio -->

    <owl:NamedIndividual rdf:about="http://www.semanticweb.org/paulagranadosgarcia/CuCoO/Mansio"/>
    


    <!-- http://www.semanticweb.org/paulagranadosgarcia/CuCoO/Material -->

    <owl:NamedIndividual rdf:about="http://www.semanticweb.org/paulagranadosgarcia/CuCoO/Material">
        <rdf:type rdf:resource="http://www.semanticweb.org/paulagranadosgarcia/CuCoO/Measure"/>
    </owl:NamedIndividual>
    


    <!-- http://www.semanticweb.org/paulagranadosgarcia/CuCoO/Metrology -->

    <owl:NamedIndividual rdf:about="http://www.semanticweb.org/paulagranadosgarcia/CuCoO/Metrology">
        <rdf:type rdf:resource="http://www.semanticweb.org/paulagranadosgarcia/CuCoO/Measure"/>
    </owl:NamedIndividual>
    


    <!-- http://www.semanticweb.org/paulagranadosgarcia/CuCoO/Military_Camp -->

    <owl:NamedIndividual rdf:about="http://www.semanticweb.org/paulagranadosgarcia/CuCoO/Military_Camp"/>
    


    <!-- http://www.semanticweb.org/paulagranadosgarcia/CuCoO/Naturalistic_style -->

    <owl:NamedIndividual rdf:about="http://www.semanticweb.org/paulagranadosgarcia/CuCoO/Naturalistic_style">
        <rdf:type rdf:resource="http://www.semanticweb.org/paulagranadosgarcia/CuCoO/Carving"/>
    </owl:NamedIndividual>
    


    <!-- http://www.semanticweb.org/paulagranadosgarcia/CuCoO/Necropolis -->

    <owl:NamedIndividual rdf:about="http://www.semanticweb.org/paulagranadosgarcia/CuCoO/Necropolis"/>
    


    <!-- http://www.semanticweb.org/paulagranadosgarcia/CuCoO/Oppidum -->

    <owl:NamedIndividual rdf:about="http://www.semanticweb.org/paulagranadosgarcia/CuCoO/Oppidum"/>
    


    <!-- http://www.semanticweb.org/paulagranadosgarcia/CuCoO/Oretani -->

    <owl:NamedIndividual rdf:about="http://www.semanticweb.org/paulagranadosgarcia/CuCoO/Oretani">
        <rdf:type rdf:resource="http://www.semanticweb.org/paulagranadosgarcia/CuCoO/EthnicIdentity"/>
    </owl:NamedIndividual>
    


    <!-- http://www.semanticweb.org/paulagranadosgarcia/CuCoO/Phoenician -->

    <owl:NamedIndividual rdf:about="http://www.semanticweb.org/paulagranadosgarcia/CuCoO/Phoenician">
        <rdf:type rdf:resource="http://www.semanticweb.org/paulagranadosgarcia/CuCoO/EthnicIdentity"/>
        <rdf:type rdf:resource="http://www.semanticweb.org/paulagranadosgarcia/CuCoO/Text"/>
    </owl:NamedIndividual>
    


    <!-- http://www.semanticweb.org/paulagranadosgarcia/CuCoO/Procedence -->

    <owl:NamedIndividual rdf:about="http://www.semanticweb.org/paulagranadosgarcia/CuCoO/Procedence"/>
    


    <!-- http://www.semanticweb.org/paulagranadosgarcia/CuCoO/Punic -->

    <owl:NamedIndividual rdf:about="http://www.semanticweb.org/paulagranadosgarcia/CuCoO/Punic">
        <rdf:type rdf:resource="http://www.semanticweb.org/paulagranadosgarcia/CuCoO/EthnicIdentity"/>
        <rdf:type rdf:resource="http://www.semanticweb.org/paulagranadosgarcia/CuCoO/Text"/>
    </owl:NamedIndividual>
    


    <!-- http://www.semanticweb.org/paulagranadosgarcia/CuCoO/Roman -->

    <owl:NamedIndividual rdf:about="http://www.semanticweb.org/paulagranadosgarcia/CuCoO/Roman">
        <rdf:type rdf:resource="http://www.semanticweb.org/paulagranadosgarcia/CuCoO/EthnicIdentity"/>
    </owl:NamedIndividual>
    


    <!-- http://www.semanticweb.org/paulagranadosgarcia/CuCoO/Sanctuary -->

    <owl:NamedIndividual rdf:about="http://www.semanticweb.org/paulagranadosgarcia/CuCoO/Sanctuary"/>
    


    <!-- http://www.semanticweb.org/paulagranadosgarcia/CuCoO/Schematic_folds -->

    <owl:NamedIndividual rdf:about="http://www.semanticweb.org/paulagranadosgarcia/CuCoO/Schematic_folds">
        <rdf:type rdf:resource="http://www.semanticweb.org/paulagranadosgarcia/CuCoO/Carving"/>
    </owl:NamedIndividual>
    


    <!-- http://www.semanticweb.org/paulagranadosgarcia/CuCoO/Settlement -->

    <owl:NamedIndividual rdf:about="http://www.semanticweb.org/paulagranadosgarcia/CuCoO/Settlement">
        <rdf:type rdf:resource="http://www.semanticweb.org/paulagranadosgarcia/CuCoO/CulturalContactAgent"/>
    </owl:NamedIndividual>
    


    <!-- http://www.semanticweb.org/paulagranadosgarcia/CuCoO/Social_Behaviour -->

    <owl:NamedIndividual rdf:about="http://www.semanticweb.org/paulagranadosgarcia/CuCoO/Social_Behaviour"/>
    


    <!-- http://www.semanticweb.org/paulagranadosgarcia/CuCoO/Text -->

    <owl:NamedIndividual rdf:about="http://www.semanticweb.org/paulagranadosgarcia/CuCoO/Text"/>
    


    <!-- http://www.semanticweb.org/paulagranadosgarcia/CuCoO/Turdetani -->

    <owl:NamedIndividual rdf:about="http://www.semanticweb.org/paulagranadosgarcia/CuCoO/Turdetani">
        <rdf:type rdf:resource="http://www.semanticweb.org/paulagranadosgarcia/CuCoO/EthnicIdentity"/>
    </owl:NamedIndividual>
    


    <!-- http://www.semanticweb.org/paulagranadosgarcia/CuCoO/Turduli -->

    <owl:NamedIndividual rdf:about="http://www.semanticweb.org/paulagranadosgarcia/CuCoO/Turduli">
        <rdf:type rdf:resource="http://www.semanticweb.org/paulagranadosgarcia/CuCoO/EthnicIdentity"/>
    </owl:NamedIndividual>
    


    <!-- http://www.semanticweb.org/paulagranadosgarcia/CuCoO/Urbanism -->

    <owl:NamedIndividual rdf:about="http://www.semanticweb.org/paulagranadosgarcia/CuCoO/Urbanism"/>
    


    <!-- 
    ///////////////////////////////////////////////////////////////////////////////////////
    //
    // Annotations
    //
    ///////////////////////////////////////////////////////////////////////////////////////
     -->

    <rdf:Description rdf:about="http://www.semanticweb.org/paulagranadosgarcia/CuCoO/Carving">
        <rdfs:comment></rdfs:comment>
    </rdf:Description>
</rdf:RDF>



<!-- Generated by the OWL API (version 4.2.8.20170104-2310) https://github.com/owlcs/owlapi -->

